prefix graph: <https://triplydb.com/Triply/yalc/graphs/>
prefix id: <https://triplydb.com/Triply/yalc/id/>
prefix owl: <http://www.w3.org/2002/07/owl#>
prefix rdf: <http://www.w3.org/1999/02/22-rdf-syntax-ns#>
prefix rdfs: <http://www.w3.org/2000/01/rdf-schema#>
prefix sdo: <http://schema.org/>
prefix time: <http://www.w3.org/2006/time#>
prefix vann: <http://purl.org/vocab/vann/>
prefix void: <http://rdfs.org/ns/void#>
prefix xsd: <http://www.w3.org/2001/XMLSchema#>
prefix yalc: <https://triplydb.com/Triply/yalc/vocab/>

<https://triplydb.com/Triply/yalc> {
  <https://triplydb.com/Triply/yalc> a void:Dataset;
    rdfs:label "LOD Cloud Catalog"@en;
    owl:versionNumber "2020.9.5";
    void:subSet graph:vocab.

  graph:vocab a owl:Ontology;
    rdfs:comment "Ontology describing the definitions (classes and properties) used in the LOD Cloud Catalog."@en;
    rdfs:label "LOD Cloud Catalog Vocabulary"@en.
}

graph:vocab {
  id:always a yalc:ChangeFrequence;
    rdfs:comment "Indicates that a resource is expected to be different every time it is accessed."@en;
    rdfs:label "Always"@en.

  id:hourly a yalc:ChangeFrequency;
    rdfs:comment "Indicates that a resource is expected to change (approximately) every hour."@en;
    rdfs:label "Hourly"@en.

  id:daily a yalc:ChangeFrequency;
    rdfs:comment "Indicates that a resource is expected to change (approximately) every day."@en;
    rdfs:label "Daily"@en.

  id:weekly a yalc:ChangeFrequency;
    rdfs:comment "Indicates that a resource is expected to change (approximately) every hour."@en;
    rdfs:label "Weekly"@en.

  id:monthly a yalc:ChangeFrequency;
    rdfs:comment "Indicates that a resource is expected to change (approximately) every hour."@en;
    rdfs:label "Monthly"@en.

  id:yearly a yalc:ChangeFrequency;
    rdfs:comment "Indicates that a resource is expected to change (approximately) every hour."@en;
    rdfs:label "Yearly"@en.

  id:never a yalc:ChangeFrequency;
    rdfs:comment "Indicates that a resource is expected to never change.  This is used for archived resources."@en;
    rdfs:label "Never"@en.

  yalc:ChangeFrequency
    owl:equivalentClass
      [ owl:oneOf (
          id:always
          id:hourly
          id:daily
          id:weekly
          id:monthly
          id:yearly
          id:never ) ];
    rdfs:comment """<p>How frequently a resource is expected to change:</p>
<dl>
  <dt>always</dt>
  <dd>The resource is expected to be different every time it is accessed.</dd>
  <dt>hourly</dt>
  <dt>daily</dt>
  <dt>weekly</dt>
  <dt>monthly</dt>
  <dt>yearly</dt>
  <dt>never</dt>
  <dd>Used for archived resources (i.e. resources that will not be changed again).</dd>
</dl>
<p>This is used only as a guide for crawlers, and is not used to determine how frequently pages are indexed.</p>"""^^rdf:HTML;
    rdfs:isDefinedBy dataset:;
    rdfs:label "change frequency"@en;
    rdfs:subClassOf owl:Thing.

  yalc:PrefixDeclaration
    rdfs:comment "A declaration that assigns an alias label to an IRI prefix.  Such declarations are often used to abbreviate long IRIs."@en ;
    rdfs:isDefinedBy dataset:;
    rdfs:label "prefix declaration"@en ;
    rdfs:subClassOf owl:Thing.

  yalc:SemanticVersion
    rdfs:comment "A version indicator that uses semantic versioning."@en;
    rdfs:label "semantic version"@en;
    rdfs:isDefinedBy dataset:;
    rdfs:seeAlso "https://semver.org"^^xsd:anyURI;
    rdfs:subClassOf yalc:Version.

  yalc:TemporalVersion
    rdfs:comment "A version indicator that uses a temporal instant."@en;
    rdfs:label "temporal version"@en;
    rdfs:isDefinedBy dataset:;
    rdfs:subClassOf
      yalc:Version,
      time:Instant.

  yalc:Version
    rdfs:comment "A version indicator."@en;
    rdfs:isDefinedBy dataset:;
    rdfs:label "version"@en;
    rdfs:subClassOf owl:Thing.

  yalc:alias a owl:DatatypeProperty;
    rdfs:comment "The alias label of the prefex declarations.  Typically, the alias label is shorter and easier to remember than the IRI prefix that is denotes."@en;
    rdfs:domain yalc:PrefixDeclaration;
    rdfs:isDefinedBy dataset:;
    rdfs:label "has alias"@en;
    rdfs:range xsd:string.

  yalc:changeFrequency a owl:ObjectProperty;
    rdfs:command "The expected change frequency for a resource."@en;
    rdfs:domain rdfs:Resource;
    rdfs:isDefinedBy dataset:;
    rdfs:label "change frequency"@en;
    rdfs:range yalc:ChangeFrequency.

  yalc:exampleResource a owl:ObjectProperty;
    rdfs:comment "An example resource that is indicative of the dataset."@en;
    rdfs:domain void:Dataset;
    rdfs:isDefinedBy dataset:;
    rdfs:label "has example resource"@en;
    rdfs:range rdfs:Resource;
    rdfs:subPropertyOf vann:example.

  yalc:major a owl:DatatypeProperty;
    rdfs:comment "The major version.  This changes when the semantics of existing data items has changed.  Changing the semantics of existing data items potentially changes the semantics of other datasets that link to this dataset."@en;
    rdfs:domain yalc:SemanticVersion;
    rdfs:isDefinedBy dataset:;
    rdfs:label "has major version"@en;
    rdfs:range xsd:nonNegativeInteger.

  yalc:minor a owl:DatatypeProperty;
    rdfs:comment "The minor version.  This changes when new data items are added without changing the semantics of existing data items.  A minor version increase does not change the semantics for other datasets that link to this dataset."@en;
    rdfs:domain yalc:SemanticVersion;
    rdfs:isDefinedBy dataset:;
    rdfs:label "has minor version"@en;
    rdfs:range xsd:nonNegativeInteger.

  yalc:namespace a owl:ObjectProperty;
    rdfs:comment "The relationship between a dataset and the IRI prefixes (or namespaces) for which the dataset is considered to be the authority."@en;
    rdfs:domain void:Dataset;
    rdfs:isDefinedBy dataset:;
    rdfs:label "has namespace"@en;
    rdfs:range xsd:anyURI.

  yalc:organization a owl:ObjectProperty;
    rdfs:comment "The relationship between a dataset and the organization that publishes it."@en;
    rdfs:domain void:Dataset;
    rdfs:isDefinedBy dataset:;
    rdfs:label "has organization"@en;
    rdfs:range sdo:Organization.

  yalc:patch a owl:DatatypeProperty;
    rdfs:comment "The patch version.  This changes when bugs in existing data items were fixed.  A patch version increase shlould always be followed by other datasets that link to this dataset, since the linked-to data entity may have contained bugs,"@en;
    rdfs:domain yalc:SemanticVersion;
    rdfs:isDefinedBy dataset:;
    rdfs:label "has patch version"@en;
    rdfs:range xsd:nonNegativeInteger.

  yalc:prefix a owl:DatatypeProperty;
    rdfs:comment "The IRI prefix of the prefix declaration."@en;
    rdfs:domain yalc:PrefixDeclaration;
    rdfs:isDefinedBy dataset:;
    rdfs:label "has prefix"@en;
    rdfs:range xsd:anyURI.

  yalc:prefixDeclaration a owl:ObjectProperty;
    rdfs:comment "Preferred prefix declarations for use with the dataset."@en;
    rdfs:domain void:Dataset;
    rdfs:isDefinedBy dataset:;
    rdfs:label "has prefix declaration"@en;
    rdfs:range yalc:PrefixDeclaration.

  yalc:version a owl:ObjectProperty;
    rdfs:comment "The relationship between a dataset and its version indicator."@en;
    rdfs:domain void:Dataset;
    rdfs:isDefinedBy dataset:;
    rdfs:label "has version"@en;
    rdfs:range yalc:Version.
}
