prefix dataset: <https://triplydb.com/Triply/yalc/>
prefix graph: <https://triplydb.com/Triply/yalc/graphs/>
prefix owl: <http://www.w3.org/2002/07/owl#>
prefix rdfs: <http://www.w3.org/2000/01/rdf-schema#>
prefix sdo: <http://schema.org/>
prefix time: <http://www.w3.org/2006/time#>
prefix void: <http://rdfs.org/ns/void#>
prefix xsd: <http://www.w3.org/2001/XMLSchema#>
prefix yalc: <https://triplydb.com/Triply/yalc/vocab/>

dataset: {
  dataset: a void:Dataset;
    rdfs:label "LOD Cloud Catalog"@en;
    owl:versionNumber "2020.03";
    void:subSet graph:vocab.

  graph:vocab a owl:Ontology;
    rdfs:comment "Ontology describing the definitions (classes and properties) used in the LOD Cloud Catalog."@en;
    rdfs:label "LOD Cloud Catalog Vocabulary"@en.
}

graph:vocab {
  yalc:Namespace
    rdfs:comment "An RDF namespace declaration."@en ;
    rdfs:isDefinedBy dataset:;
    rdfs:label "namespace"@en ;
    rdfs:subClassOf owl:Thing.

  yalc:SemanticVersion
    rdfs:comment "A version indicator that uses semantic versioning."@en;
    rdfs:label "semantic version"@en;
    rdfs:isDefinedBy dataset:;
    rdfs:seeAlso "https://semver.org"^^xsd:anyURI;
    rdfs:subClassOf yalc:Version.

  yalc:TemporalVersion
    rdfs:comment "A version indicator that uses a temporal instant."@en;
    rdfs:label "temporal version"@en;
    rdfs:isDefinedBy dataset:;
    rdfs:subClassOf
      yalc:Version,
      time:Instant.

  yalc:Version
    rdfs:comment "A version indicator."@en;
    rdfs:isDefinedBy dataset:;
    rdfs:label "version"@en;
    rdfs:subClassOf owl:Thing.

  yalc:alias a owl:DatatypeProperty;
    rdfs:comment "The alias that will be used to denote the namespace.  Typically, the alias is shorter and easier to remember than the IRI prefix that is stands for."@en;
    rdfs:domain yalc:Namespace;
    rdfs:isDefinedBy dataset:;
    rdfs:label "has alias"@en;
    rdfs:range xsd:string.

  yalc:exampleResource
    rdfs:comment "An example resource that is indicative of the dataset."@en;
    rdfs:domain void:Dataset;
    rdfs:isDefinedBy dataset:;
    rdfs:label "has example resource"@en;
    rdfs:range xsd:anyURI.

  yalc:major a owl:DatatypeProperty;
    rdfs:comment "The major version.  This changes when the semantics of existing data items has changed.  Changing the semantics of existing data items potentially changes the semantics of other datasets that link to this dataset."@en;
    rdfs:domain yalc:SemanticVersion;
    rdfs:isDefinedBy dataset:;
    rdfs:label "has major version"@en;
    rdfs:range xsd:nonNegativeInteger.

  yalc:minor a owl:DatatypeProperty;
    rdfs:comment "The minor version.  This changes when new data items are added without changing the semantics of existing data items.  A minor version increase does not change the semantics for other datasets that link to this dataset."@en;
    rdfs:domain yalc:SemanticVersion;
    rdfs:isDefinedBy dataset:;
    rdfs:label "has minor version"@en;
    rdfs:range xsd:nonNegativeInteger.

  yalc:namespace a owl:ObjectProperty;
    rdfs:comment "The relationship between a dataset and a preferred namespace for that dataset."@en;
    rdfs:domain void:Dataset;
    rdfs:isDefinedBy dataset:;
    rdfs:label "has namespace"@en;
    rdfs:range yalc:Namespace.

  yalc:organization a owl:ObjectProperty;
    rdfs:comment "The relationship between a dataset and the organization that publishes it."@en;
    rdfs:domain void:Dataset;
    rdfs:isDefinedBy dataset:;
    rdfs:label "has organization"@en;
    rdfs:range sdo:Organization.

  yalc:patch a owl:DatatypeProperty;
    rdfs:comment "The patch version.  This changes when bugs in existing data items were fixed.  A patch version increase shlould always be followed by other datasets that link to this dataset, since the linked-to data entity may have contained bugs,"@en;
    rdfs:domain yalc:SemanticVersion;
    rdfs:isDefinedBy dataset:;
    rdfs:label "has patch version"@en;
    rdfs:range xsd:nonNegativeInteger.

  yalc:prefix a owl:DatatypeProperty;
    rdfs:comment "The IRI prefix of the namespace."@en;
    rdfs:domain yalc:Namespace;
    rdfs:isDefinedBy dataset:;
    rdfs:label "has prefix"@en;
    rdfs:range xsd:anyURI.

  yalc:version a owl:ObjectProperty;
    rdfs:comment "The relationship between a dataset and its version indicator."@en;
    rdfs:domain void:Dataset;
    rdfs:isDefinedBy dataset:;
    rdfs:label "has version"@en;
    rdfs:range yalc:Version.
}
